Improve exception handling and propagation

shift-reset/core/syntax.v
@@ -21,15 +21,20 @@ Inductive prim2 : Type :=
 | P2Eq : prim2
 | P2Neq : prim2.
 
-Inductive binder : Type :=
-| BAnon : binder
-| BVar : ident -> binder.
-
 Inductive atom : Type :=
 | AUnit : atom
 | AInt : Z -> atom
 | ABool : bool -> atom
 | AVar : ident -> atom.
+
+Inductive binder : Type :=
+| BAny : binder
+| BVar : ident -> binder.
+
+Inductive exn_pattern : Type :=
+| ExnPAny : exn_pattern
+| ExnPVar : ident -> exn_pattern
+| ExnPExn : ident -> ident -> exn_pattern.
 
 Inductive term : Type :=
 | TAtom : atom -> term
@@ -55,11 +60,13 @@ Inductive term : Type :=
 | TPrompt : term -> term
 | TExn : ident -> atom -> term
 | TRaise : atom -> term
-| TTry : term -> ident -> term1 -> term
+| TTry : term -> exn_term -> term
 with term1 : Type :=
 | T1 : binder -> term -> term1
 with term2 : Type :=
-| T2 : binder -> binder -> term -> term2.
+| T2 : binder -> binder -> term -> term2
+with exn_term : Type :=
+| ExnT : exn_pattern -> term -> exn_term.
 
 Inductive val : Type :=
 | VUnit : val
@@ -78,60 +85,84 @@ with clo1 : Type :=
 | C1 : env -> term1 -> clo1
 with clo2 : Type :=
 | C2 : env -> term2 -> clo2
+with exn_clo : Type :=
+| ExnC : env -> exn_term -> exn_clo
 with kont1 : Type :=
 | K1Nil : kont1
 | K1Cons : clo1 -> kont1 -> kont1
 with kont2S : Type :=
-| K2SHead : kont1 -> kont2S
-| K2SSnoc : kont2S -> kont1 -> kont2S
+| K2SPure : kont1 -> kont2S
+| K2SPrompt : kont2S -> kont1 -> kont2S
+| K2STry : kont2S -> exn_clo -> kont1 -> kont2S
 with kont2C : Type :=
-| K2CHead : kont1 -> kont2C
-| K2CSnoc : kont2C -> kont1 -> kont2C
+| K2CPure : kont1 -> kont2C
+| K2CReset : kont2C -> kont1 -> kont2C
+| K2CTry : kont2C -> exn_clo -> kont1 -> kont2C
 with env : Type :=
 | EnvNil : env
 | EnvCons : ident -> val -> env -> env
 with exn : Type :=
 | Exn : ident -> val -> exn.
 
+Create HintDb eq_dec_db discriminated.
+
+Hint Resolve Z.eq_dec : eq_dec_db.
+Hint Resolve bool_dec : eq_dec_db.
+Hint Resolve ident_eq_dec : eq_dec_db.
+Hint Resolve loc_eq_dec : eq_dec_db.
+
 Definition prim1_eq_dec : forall (p1 p2 : prim1), {p1 = p2} + {p1 <> p2}.
-Proof. decide equality. Defined.
+Proof. decide equality; auto with eq_dec_db. Defined.
 
 Definition prim2_eq_dec : forall (p1 p2 : prim2), {p1 = p2} + {p1 <> p2}.
-Proof. decide equality. Defined.
-
-Definition binder_eq_dec : forall (b1 b2 : binder), {b1 = b2} + {b1 <> b2}.
-Proof. decide equality; auto using ident_eq_dec. Defined.
+Proof. decide equality; auto with eq_dec_db. Defined.
 
 Definition atom_eq_dec : forall (a1 a2 : atom), {a1 = a2} + {a1 <> a2}.
-Proof. decide equality; auto using Z.eq_dec, bool_dec, ident_eq_dec. Defined.
+Proof. decide equality; auto with eq_dec_db. Defined.
+
+Definition binder_eq_dec : forall (b1 b2 : binder), {b1 = b2} + {b1 <> b2}.
+Proof. decide equality; auto with eq_dec_db. Defined.
+
+Definition exn_pattern_eq_dec : forall (p1 p2 : exn_pattern), {p1 = p2} + {p1 <> p2}.
+Proof. decide equality; auto with eq_dec_db. Defined.
+
+Hint Resolve prim1_eq_dec : eq_dec_db.
+Hint Resolve prim2_eq_dec : eq_dec_db.
+Hint Resolve atom_eq_dec : eq_dec_db.
+Hint Resolve binder_eq_dec : eq_dec_db.
+Hint Resolve exn_pattern_eq_dec : eq_dec_db.
 
 Fixpoint term_eq_dec : forall (t1 t2 : term), {t1 = t2} + {t1 <> t2}
 with term1_eq_dec : forall (t1 t2 : term1), {t1 = t2} + {t1 <> t2}
-with term2_eq_dec : forall (t1 t2 : term2), {t1 = t2} + {t1 <> t2}.
-Proof.
-  { decide equality; auto using atom_eq_dec, prim1_eq_dec, prim2_eq_dec, ident_eq_dec. }
-  { decide equality; auto using binder_eq_dec. }
-  { decide equality; auto using binder_eq_dec. }
-Defined.
+with term2_eq_dec : forall (t1 t2 : term2), {t1 = t2} + {t1 <> t2}
+with exn_term_eq_dec : forall (t1 t2 : exn_term), {t1 = t2} + {t1 <> t2}.
+Proof. all: decide equality; auto with eq_dec_db. Defined.
+
+Hint Resolve term_eq_dec : eq_dec_db.
+Hint Resolve term1_eq_dec : eq_dec_db.
+Hint Resolve term2_eq_dec : eq_dec_db.
+Hint Resolve exn_term_eq_dec : eq_dec_db.
 
 Fixpoint val_eq_dec : forall (v1 v2 : val), {v1 = v2} + {v1 <> v2}
 with clo1_eq_dec : forall (c1 c2 : clo1), {c1 = c2} + {c1 <> c2}
 with clo2_eq_dec : forall (c1 c2 : clo2), {c1 = c2} + {c1 <> c2}
+with exn_clo_eq_dec : forall (c1 c2 : exn_clo), {c1 = c2} + {c1 <> c2}
 with kont1_eq_dec : forall (k1 k2 : kont1), {k1 = k2} + {k1 <> k2}
 with kont2S_eq_dec : forall (ks1 ks2 : kont2S), {ks1 = ks2} + {ks1 <> ks2}
 with kont2C_eq_dec : forall (kc1 kc2 : kont2C), {kc1 = kc2} + {kc1 <> kc2}
 with env_eq_dec : forall (env1 env2 : env), {env1 = env2} + {env1 <> env2}
 with exn_eq_dec : forall (exn1 exn2 : exn), {exn1 = exn2} + {exn1 <> exn2}.
-Proof.
-  { decide equality; auto using Z.eq_dec, bool_dec, loc_eq_dec. }
-  { decide equality; auto using term1_eq_dec. }
-  { decide equality; auto using term2_eq_dec. }
-  { decide equality. }
-  { decide equality. }
-  { decide equality. }
-  { decide equality; auto using ident_eq_dec. }
-  { decide equality; auto using ident_eq_dec. }
-Defined.
+Proof. all: decide equality; auto with eq_dec_db. Defined.
+
+Hint Resolve val_eq_dec : eq_dec_db.
+Hint Resolve clo1_eq_dec : eq_dec_db.
+Hint Resolve clo2_eq_dec : eq_dec_db.
+Hint Resolve exn_clo_eq_dec : eq_dec_db.
+Hint Resolve kont1_eq_dec : eq_dec_db.
+Hint Resolve kont2S_eq_dec : eq_dec_db.
+Hint Resolve kont2C_eq_dec : eq_dec_db.
+Hint Resolve env_eq_dec : eq_dec_db.
+Hint Resolve exn_eq_dec : eq_dec_db.
 
 Definition val_eqb (v1 v2 : val) : bool := if val_eq_dec v1 v2 then true else false.
 Definition val_neqb (v1 v2 : val) : bool := if val_eq_dec v1 v2 then false else true.
